theories/Examples/Mu/PolarizedSystemL.v
@@ -2,7 +2,8 @@ From OGS Require Import Prelude.
 From OGS.Utils Require Import Psh Rel Ctx.
 From OGS.Game Require Import Event.
 From OGS.ITree Require Import ITree Eq Delay Structure Properties.
-Set Equations Transparent.
+Declare Scope ty_scope .
+From OGS.OGS Require Import Soundness.
 
 Variant pol : Type := pos | neg .
 Derive NoConfusion for pol.
@@ -111,21 +112,21 @@ Equations v_rename {Γ Δ} : Γ ⊆ Δ -> val Γ ⇒ᵢ val Δ :=
 Definition a_ren {Γ1 Γ2 Γ3} : Γ2 ⊆ Γ3 -> Γ1 =[val]> Γ2 -> Γ1 =[val]> Γ3 :=
   fun f g _ i => v_rename f _ (g _ i) .
 
-Definition t_shift  {Γ} [y] : term Γ ⇒ᵢ term (Γ ▶ y)  := @t_rename _ _ s_pop.
-Definition w_shift {Γ} [y] : whn Γ ⇒ᵢ whn (Γ ▶ y)  := @w_rename _ _ s_pop.
-Definition s_shift  {Γ} [y] : state Γ -> state (Γ ▶ y) := @s_rename _ _ s_pop.
-Definition v_shift  {Γ} [y] : val Γ ⇒ᵢ val (Γ ▶ y)    := @v_rename _ _ s_pop.
-Definition v_shift2  {Γ} [y z] : val Γ ⇒ᵢ val (Γ ▶ y ▶ z)  := @v_rename _ _ (s_pop ⊛ᵣ s_pop).
-Definition v_shift3  {Γ} [x y z] : val Γ ⇒ᵢ val (Γ ▶ x ▶ y ▶ z)  := @v_rename _ _ (s_pop ⊛ᵣ s_pop ⊛ᵣ s_pop).
+Definition t_shift  {Γ} [y] : term Γ ⇒ᵢ term (Γ ▶ y)  := @t_rename _ _ r_pop.
+Definition w_shift {Γ} [y] : whn Γ ⇒ᵢ whn (Γ ▶ y)  := @w_rename _ _ r_pop.
+Definition s_shift  {Γ} [y] : state Γ -> state (Γ ▶ y) := @s_rename _ _ r_pop.
+Definition v_shift  {Γ} [y] : val Γ ⇒ᵢ val (Γ ▶ y)    := @v_rename _ _ r_pop.
+Definition v_shift2  {Γ} [y z] : val Γ ⇒ᵢ val (Γ ▶ y ▶ z)  := @v_rename _ _ (r_pop ⊛ᵣ r_pop).
+Definition v_shift3  {Γ} [x y z] : val Γ ⇒ᵢ val (Γ ▶ x ▶ y ▶ z)  := @v_rename _ _ (r_pop ⊛ᵣ r_pop ⊛ᵣ r_pop).
 
 Definition a_shift {Γ Δ} [y] (a : Γ =[val]> Δ) : (Γ ▶ y) =[val]> (Δ ▶ y) :=
-  s_append (fun _ i => v_shift _ (a _ i)) (s_var _ top).
+  a_append (fun _ i => v_shift _ (a _ i)) (s_var _ top).
 
 Definition a_shift2 {Γ Δ} [y z] (a : Γ =[val]> Δ) : (Γ ▶ y ▶ z) =[val]> (Δ ▶ y ▶ z) :=
-  s_append (s_append (fun _ i => v_shift2 _ (a _ i)) (s_var _ (pop (top)))) (s_var _ top).
+  a_append (a_append (fun _ i => v_shift2 _ (a _ i)) (s_var _ (pop (top)))) (s_var _ top).
 
 Definition a_shift3 {Γ Δ} [x y z] (a : Γ =[val]> Δ) : (Γ ▶ x ▶ y ▶ z) =[val]> (Δ ▶ x ▶ y ▶ z) :=
-  s_append (s_append (s_append (fun _ i => v_shift3 _ (a _ i))
+  a_append (a_append (a_append (fun _ i => v_shift3 _ (a _ i))
                         (s_var _ (pop (pop top))))
               (s_var _ (pop top)))
     (s_var _ top).
@@ -183,7 +184,7 @@ Definition App'' {Γ a b} (f : term Γ (t+ (a → b))) (x : term Γ (t+ a)) : te
 
 (*
 Definition Ram' {Γ a b} (u : term (Γ ▶ t+ a) (t+ b)) : whn Γ (a → b) :=
-  RamLec (t_rename (r_shift s_pop) (t+ _) u) . 
+  RamLec (t_rename (r_shift r_pop) (t+ _) u) . 
 
 Definition ty_nat (a : ty0) : ty0 := (a → ((a → a) → a)) .
 Definition nat_ze {a} : term ∅ (t+ ty_nat a) :=
@@ -245,7 +246,7 @@ Equations v_subst {Γ Δ} : Γ =[val]> Δ -> val Γ ⇒ᵢ val Δ :=
 Definition a_comp {Γ1 Γ2 Γ3} : Γ2 =[val]> Γ3 -> Γ1 =[val]> Γ2 -> Γ1 =[val]> Γ3 :=
   fun f g _ i => v_subst f _ (g _ i) .
 
-Definition ass1 {Γ a} (v : val Γ a) : (Γ ▶ a) =[val]> Γ := s_append s_var v .
+Definition ass1 {Γ a} (v : val Γ a) : (Γ ▶ a) =[val]> Γ := a_append s_var v .
 
 Definition t_subst1 {Γ a b} u v := t_subst (@ass1 Γ a v) b u.
 Definition w_subst1 {Γ a b} u v := w_subst (@ass1 Γ a v) b u.
@@ -349,18 +350,18 @@ Equations p_dom_of_w_0p {Γ : neg_ctx} (A : ty0 pos) (v : whn Γ (t+ A)) : p_dom
   p_dom_of_w_0p (↓ A)  (Var i) with (s_elt_upg i).(sub_prf) := { | ! } ;
   p_dom_of_w_0p (A ⊕ B) (OrR1 v)     := p_dom_of_w_0p A v ;
   p_dom_of_w_0p (A ⊕ B) (OrR2 v)     := p_dom_of_w_0p B v ;
-  p_dom_of_w_0p (↓ A)  (ShiftPR x)  := s_append s_empty x ;
+  p_dom_of_w_0p (↓ A)  (ShiftPR x)  := a_append a_empty x ;
 with p_dom_of_w_0n {Γ : neg_ctx} (A : ty0 neg) (k : whn Γ (t- A)) : p_dom (p_of_w_0n A k) =[val]> Γ by struct A :=
   p_dom_of_w_0n (B-) (Var i) with (s_elt_upg i).(sub_prf) := { | ! } ;
   p_dom_of_w_0n (A → B) (Var i) with (s_elt_upg i).(sub_prf) := { | ! } ;
   p_dom_of_w_0n (↑ A)  (Var i) with (s_elt_upg i).(sub_prf) := { | ! } ;
   p_dom_of_w_0n (A → B) (ArrL v k) := [ p_dom_of_w_0p A v , p_dom_of_w_0n B k ] ;
-  p_dom_of_w_0n (↑ A)  (ShiftNL x)  := s_append s_empty x .
+  p_dom_of_w_0n (↑ A)  (ShiftNL x)  := a_append a_empty x .
 
 Equations p_dom_of_v {Γ : neg_ctx} A (v : val Γ A) : p_dom (p_of_v A v) =[val]> Γ :=
   p_dom_of_v (@VTy pos A) v := p_dom_of_w_0p A v ;
-  p_dom_of_v (@KTy pos A) x := s_append s_empty x ;
-  p_dom_of_v (@VTy neg A) x := s_append s_empty x ;
+  p_dom_of_v (@KTy pos A) x := a_append a_empty x ;
+  p_dom_of_v (@VTy neg A) x := a_append a_empty x ;
   p_dom_of_v (@KTy neg A) k := p_dom_of_w_0n A k .
 
 Definition nf0 (Γ : t_ctx) (A : ty) : Type := sigT (fun p : pat (t_neg A) => p_dom p =[val]> Γ) .
@@ -634,7 +635,7 @@ Lemma a_shift_a_ren {Γ1 Γ2 Γ3 y} (f1 : Γ2 ⊆ Γ3) (f2 : Γ1 =[ val ]> Γ2)
   unfold r_shift, a_shift, a_ren, v_shift; intros ? h.
   dependent elimination h; cbn.
   - now rewrite v_ren_id_r.
-  - now rewrite 2 v_ren_ren, s_append_pop.
+  - now rewrite 2 v_ren_ren, a_append_pop.
 Qed.
 
 Lemma a_shift_s_ren {Γ1 Γ2 Γ3 y} (f1 : Γ2 =[val]> Γ3) (f2 : Γ1 ⊆ Γ2)
@@ -1028,11 +1029,6 @@ Lemma then_eval_eq {Γ Δ : neg_ctx} (e : Γ =[val]> Δ) (n : nf Γ) : then_eval
   now rewrite <- w_sub_sub.
 Qed.
 
-(* we can prove the hypothesis:
-
-    eval (c / e) == eval c >>= λ n => eval (⌊ n ⌋ / e)
-*)
-
 Lemma fmap_comp_eq {Γ} {u v : delay (nf Γ)} : u ≋ v -> fmap_delay (pat_of_nf Γ) u ≊ fmap_delay (pat_of_nf Γ) v .
   intro H.
   unfold it_eq; revert u v H; coinduction L CIH; intros u v H.
@@ -1047,100 +1043,6 @@ Lemma fmap_comp_eq {Γ} {u v : delay (nf Γ)} : u ≋ v -> fmap_delay (pat_of_nf
   now rewrite H2,H3.
   destruct q.
 Qed.
-(*
-Lemma clean_hyp {Γ Δ : neg_ctx} (c : state Γ) (e : Γ ⊆ Δ)
-   : eval (s_rename e c) ≊ fmap_delay (n_rename e) (eval c) .
-  unfold it_eq; revert Γ c e; coinduction L CIH; intros Γ c e.
-  cbn.
-  dependent elimination c.
-  dependent elimination t0.
-  - cbn; econstructor. (* Cut (Mu _) _) *)
-    change (t_rename e (t- a0) t1) with (v_rename e (t- a0) t1).
-    rewrite s_sub1_ren.
-    apply CIH.
-  - dependent elimination t1.
-    + cbn; econstructor. unfold n_rename; cbn.
-      do 2 f_equal.
-      rewrite p_of_v_eq.
-      unfold a_ren.
-      ; reflexivity. cbn. rewrite s_subst_equation_1, t_subst_equation_3.
-      unfold eval at 2; cbn -[eval then_eval2].
-      unfold then_eval2.
-      cbn -[eval eval_aux]; rewrite refold_id.
-      cbv [observe]; destruct (_observe (eval (Cut (Val (w_subst e a2 v)) (e (t- a2) h)))); econstructor; reflexivity.
-    + unfold eval. cbn -[then_eval2]; change (iter _ T1_0 ?x) with (eval x).
-      change (w_subst e a3 v) with (v_subst e (t+ a3) v); rewrite s_sub1_sub.
-      econstructor; apply CIH.
-    + dependent elimination v. (* Cut (Val _) ZerK *)
-      pose (nope := (s_elt_upg h).(sub_prf)); dependent elimination nope.
-    + dependent elimination v. (* Cut (Val _) (App _ _)) *)
-      * unfold eval at 2; cbn -[eval then_eval2].
-        unfold then_eval2; cbn -[eval eval_aux].
-        rewrite w_sub_ren.
-        assert ((@s_append _ _ _ _ (t- b) (p_dom_of_v0 a4 v1) t0 ⊛ᵣ s_pop)
-                ≡ₐ p_dom_of_v0 a4 v1) by auto.
-        rewrite (w_sub_eq _ _ H a4 _ _ eq_refl), refold_id.
-        cbn -[eval_aux];
-          destruct (eval_aux (Cut (Val (e _ h)) (App (w_subst e _ v1) (t_subst e _ t0))));
-          econstructor;
-          reflexivity.
-      * cbn; econstructor; change (iter _ T1_0 ?x) with (eval x).
-        change (RamLec (t_subst (a_shift2 e) (t+ b2) t1)) with (w_subst e (a2 → b2) (RamLec t1)).
-        unfold t_subst1 at 1 2.
-        rewrite 2 t_sub_sub.
-        rewrite <- (t_sub_eq _ _ (a_comp_assoc _ _ _) (t+ b2) t1 t1 eq_refl).
-        rewrite <- t_sub_sub.
-        unfold w_shift at 1; rewrite w_ren_sub.
-        assert (a_comp (ass1 (v_subst (a_ren (s_pop (x:= (t+ (a2 → b2)))) e) (t+ a2) v1)) (a_shift2 e) ≡ₐ a_comp (a_shift e) (ass1 (v_shift (t+ _) v1))).
-        ** intros ? i; dependent elimination i as [ Ctx.top | Ctx.pop Ctx.top | Ctx.pop (Ctx.pop i) ]; cbn.
-           ++ rewrite w_sub_ren; now apply w_sub_eq.
-           ++ reflexivity.
-           ++ destruct x1; cbn.
-              rewrite w_ren_ren, w_sub_ren.
-              rewrite <- (w_sub_id_l t (w_rename s_pop t (e _ i))), w_sub_ren.
-              now apply w_sub_eq.
-              rewrite t_ren_ren, t_sub_ren.
-              rewrite <- (t_sub_id_l _ (t_rename s_pop _ (e _ i))), t_sub_ren.
-              now apply t_sub_eq.
-        ** rewrite (t_sub_eq _ _ H _ _ _ eq_refl).
-           rewrite t_sub_sub.
-        rewrite (t_sub_eq _ _ (a_comp_assoc _ _ _) (t+ b2) t1 t1 eq_refl).
-        rewrite <- t_sub_sub.
-        change (w_subst e _ (RamLec t1)) with (v_subst e (t+ _) (RamLec t1)).
-        rewrite (t_sub_eq _ _ (sub1_sub (a:=t+ _) e (RamLec t1)) _ _ _ eq_refl).
-        rewrite <- t_sub_sub.
-        change (Cut (t_subst e _ ?a) (t_subst e _ t0)) with (s_subst e (Cut a t0)).
-        apply CIH.
-    + dependent elimination v. (* Cut (Val _) Fst *)
-      * unfold eval at 2; cbn -[eval then_eval2].
-        unfold then_eval2; cbn -[eval eval_aux].
-        cbn -[eval_aux];
-          destruct (eval_aux (Cut (Val (e _ h)) (Fst (t_subst e _ t1))));
-          econstructor;
-          reflexivity.
-      * cbn; econstructor; apply CIH.
-    + dependent elimination v. (* Cut (Val _) Snd *)
-      * unfold eval at 2; cbn -[eval then_eval2].
-        unfold then_eval2; cbn -[eval eval_aux].
-        cbn -[eval_aux];
-          destruct (eval_aux (Cut (Val (e _ h)) (Snd (t_subst e _ t2))));
-          econstructor;
-          reflexivity.
-      * cbn; econstructor; apply CIH.
-    + dependent elimination v. (* Cut (Val _) (Match _ _) *)
-      * pose (nope := (s_elt_upg h).(sub_prf)); dependent elimination nope.
-      * cbn; econstructor; change (iter _ T1_0 ?x) with (eval x).
-        change (w_subst e a0 v) with (v_subst e (t+ a0) v); rewrite s_sub1_sub.
-        apply CIH.
-      * cbn; econstructor; change (iter _ T1_0 ?x) with (eval x).
-        change (w_subst e b0 v0) with (v_subst e (t+ b0) v0); rewrite s_sub1_sub.
-        apply CIH.
-Qed.
-  - 
-    unfold 
-    rewrite s_ren1_sub.
-    apply CIH.
-    *)
 
 Lemma clean_hyp {Γ Δ : neg_ctx} (c : state Γ) (e : Γ =[val]> Δ)
    : eval (s_subst e c) ≊ bind_delay' (eval c) (then_eval1 e) .
@@ -1231,26 +1133,6 @@ Lemma is_var_dec {Γ A} (v : val Γ A) : is_var v + (is_var v -> False) .
   all: try now (apply inr; intros [ i H ]; inversion H).
   all: apply inl; econstructor; auto.
 Qed.
-
-(*
-Lemma v_is_var_ren {Γ1 Γ2 x} (v : val Γ1 x) (e : Γ1 ⊆ Γ2) : is_var (v_rename e _ v) -> is_var v .
-  intros [ i H ].
-  destruct x; cbn in *.
-  - dependent induction v; cbn in *; try now inversion H.
-    exact (h ,' eq_refl).
-  - dependent induction v; cbn in *; try now inversion H.
-    exact (h ,' eq_refl).
-Qed.
-
-Lemma v_is_var_sub {Γ1 Γ2 x} (v : val Γ1 x) (e : Γ1 ⊆ Γ2) : is_var (v_subst (Var ⊛ᵣ e) _ v) -> is_var v .
-  intros [ i H ].
-  destruct x; cbn in *.
-  - dependent induction v; cbn in *; try now inversion H.
-    exact (h ,' eq_refl).
-  - dependent induction v; cbn in *; try now inversion H.
-    exact (h ,' eq_refl).
-Qed.
-*)
 
 Equations p_of_w_eq_aux_p {Γ : neg_ctx} (A : ty0 pos) (p : pat (t+ A)) (e : p_dom p =[val]> Γ)
           : p_of_w_0p A (w_subst e (t+ A) (w_of_p p) : whn Γ (t+ A)) = p
@@ -1452,8 +1334,8 @@ Variant head_inst_nostep (u : sigT (fun A => pat (t_neg A))) : sigT (fun A => pa
 Lemma eval_app_not_var : well_founded head_inst_nostep .
   intros A; econstructor; intros [ B m ] H; dependent elimination H; cbn in *.
   destruct A0 as [ [] | [] ].
+  1,3: cycle 1.
   all: dependent elimination v; try now destruct (p (_ ,' eq_refl)).
-  all: clear p.
   all: dependent elimination m0; cbn in H.
   all: match goal with
        | u : assignment _ (neg_c_coe (p_dom (PVarN _))) _ |- _ =>
@@ -1475,172 +1357,37 @@ Lemma eval_app_not_var : well_founded head_inst_nostep .
            [ apply it_eq_step in H; cbn in H; now inversion H | ]
        | _ => idtac
        end.
-  - dependent elimination w.
-    * apply it_eq_step in H; cbn in H.
-      simp eval_aux in H.
-      dependent elimination H; cbn in r_rel.
-      inversion_sigma r_rel as [ H1 H2 ].
-      revert m i H2; rewrite <- H1; intros m i H2.
-      inversion_clear H2; cbn; clear.
-      econstructor; intros [ A p ] H; dependent elimination H; cbn in *.
-      dependent elimination v.
-      + apply it_eq_step in H; now inversion H.
-      + dependent elimination w.
-        now destruct (p0 (_ ,' eq_refl)).
-        apply it_eq_step in H; now inversion H.
-    * apply it_eq_step in H; now inversion H.
-  - dependent elimination w.
-    * apply it_eq_step in H; cbn in H.
-      simp eval_aux in H.
-      dependent elimination H; cbn in r_rel.
-      inversion_sigma r_rel as [ H1 H2 ].
-      revert m i H2; rewrite <- H1; intros m i H2.
-      inversion_clear H2; cbn; clear.
-      econstructor; intros [ A p ] H; dependent elimination H; cbn in *.
-      dependent elimination v.
-      + apply it_eq_step in H; now inversion H.
-      + dependent elimination w.
-        now destruct (p0 (_ ,' eq_refl)).
-        apply it_eq_step in H; now inversion H.
-    * apply it_eq_step in H; now inversion H.
-  - dependent elimination w.
-    * apply it_eq_step in H; cbn in H.
-      simp eval_aux in H.
-      dependent elimination H; cbn in r_rel.
-      inversion_sigma r_rel as [ H1 H2 ].
-      revert m i H2; rewrite <- H1; intros m i H2.
-      inversion_clear H2; cbn; clear.
-      econstructor; intros [ A p ] H; dependent elimination H; cbn in *.
-      dependent elimination v.
-      + apply it_eq_step in H; now inversion H.
-      + dependent elimination w.
-        now destruct (p0 (_ ,' eq_refl)).
-        apply it_eq_step in H; now inversion H.
-    * apply it_eq_step in H; now inversion H.
-  - apply it_eq_step in H; now inversion H.
-  - apply it_eq_step in H; now inversion H.
-  - dependent elimination w.
-    * apply it_eq_step in H; cbn in H.
-      simp eval_aux in H.
-      dependent elimination H; cbn in r_rel.
-      inversion_sigma r_rel as [ H1 H2 ].
-      revert m i H2; rewrite <- H1; intros m i H2.
-      inversion_clear H2; cbn; clear.
-      econstructor; intros [ A p1 ] H; dependent elimination H; cbn in *.
-      dependent elimination v.
-      + apply it_eq_step in H; now inversion H.
-      + dependent elimination w.
-        now destruct (p2 (_ ,' eq_refl)).
-        apply it_eq_step in H; now inversion H.
-    * apply it_eq_step in H; now inversion H.
-  - dependent elimination w.
-    * apply it_eq_step in H; cbn in H.
-      simp eval_aux in H.
-      dependent elimination H; cbn in r_rel.
-      inversion_sigma r_rel as [ H1 H2 ].
-      revert m i H2; rewrite <- H1; intros m i H2.
-      inversion_clear H2; cbn; clear.
-      econstructor; intros [ A p ] H; dependent elimination H; cbn in *.
-      dependent elimination v.
-      + apply it_eq_step in H; now inversion H.
-      + dependent elimination w.
-        now destruct (p0 (_ ,' eq_refl)).
-        apply it_eq_step in H; now inversion H.
-    * apply it_eq_step in H; now inversion H.
-  - apply it_eq_step in H; now inversion H.
-  - apply it_eq_step in H; now inversion H.
-  - apply it_eq_step in H; now inversion H.
-  - dependent elimination w.
-    * apply it_eq_step in H; cbn in H.
-      simp eval_aux in H.
-      dependent elimination H; cbn in r_rel.
-      inversion_sigma r_rel as [ H1 H2 ].
-      revert m i H2; rewrite <- H1; intros m i H2.
-      inversion_clear H2; cbn; clear.
-      econstructor; intros [ A p ] H; dependent elimination H; cbn in *.
-      dependent elimination v.
-      + apply it_eq_step in H; now inversion H.
-      + dependent elimination w.
-        now destruct (p0 (_ ,' eq_refl)).
-        apply it_eq_step in H; now inversion H.
-    * apply it_eq_step in H; now inversion H.
-  - dependent elimination w.
-    * apply it_eq_step in H; cbn in H.
-      simp eval_aux in H.
-      dependent elimination H; cbn in r_rel.
-      inversion_sigma r_rel as [ H1 H2 ].
-      revert m i H2; rewrite <- H1; intros m i H2.
-      inversion_clear H2; cbn; clear.
-      econstructor; intros [ A p ] H; dependent elimination H; cbn in *.
-      dependent elimination v.
-      + apply it_eq_step in H; now inversion H.
-      + dependent elimination w.
-        now destruct (p0 (_ ,' eq_refl)).
-        apply it_eq_step in H; now inversion H.
-    * apply it_eq_step in H; now inversion H.
-  - dependent elimination w.
-    * apply it_eq_step in H; cbn in H.
-      simp eval_aux in H.
-      dependent elimination H; cbn in r_rel.
-      inversion_sigma r_rel as [ H1 H2 ].
-      revert m i H2; rewrite <- H1; intros m i H2.
-      inversion_clear H2; cbn; clear.
-      econstructor; intros [ A p ] H; dependent elimination H; cbn in *.
-      dependent elimination v.
-      + apply it_eq_step in H; now inversion H.
-      + dependent elimination w.
-        now destruct (p0 (_ ,' eq_refl)).
-        apply it_eq_step in H; now inversion H.
-    * apply it_eq_step in H; now inversion H.
-  - dependent elimination w1.
-    * apply it_eq_step in H; cbn in H.
-      simp eval_aux in H.
-      dependent elimination H; cbn in r_rel.
-      inversion_sigma r_rel as [ H1 H2 ].
-      revert m i H2; rewrite <- H1; intros m i H2.
-      inversion_clear H2; cbn; clear.
-      econstructor; intros [ A p ] H; dependent elimination H; cbn in *.
-      dependent elimination v.
-      + apply it_eq_step in H; now inversion H.
-      + dependent elimination w1.
-        now destruct (p0 (_ ,' eq_refl)).
-        apply it_eq_step in H; now inversion H.
-    * apply it_eq_step in H; now inversion H.
-  - dependent elimination w.
-    * apply it_eq_step in H; cbn in H.
-      simp eval_aux in H.
-      dependent elimination H; cbn in r_rel.
-      inversion_sigma r_rel as [ H1 H2 ].
-      revert m i H2; rewrite <- H1; intros m i H2.
-      inversion_clear H2; cbn; clear.
-      econstructor; intros [ A p ] H; dependent elimination H; cbn in *.
-      dependent elimination v.
-      + apply it_eq_step in H; now inversion H.
-      + dependent elimination w.
-        now destruct (p0 (_ ,' eq_refl)).
-        apply it_eq_step in H; now inversion H.
-    * apply it_eq_step in H; now inversion H.
+  cbn in H.
+  1-3, 10-11: apply it_eq_step in H; now inversion H.
+  1-6: match goal with
+       | w : whn _ (t- _) |- _ =>
+           dependent elimination w;
+           [ | apply it_eq_step in H; now inversion H ];
+           try now destruct (p (_ ,' eq_refl))
+       | _ => idtac
+       end.
+  3-7: match goal with
+       | w : whn _ (t+ _) |- _ =>
+           dependent elimination w;
+           [ | apply it_eq_step in H; now inversion H ];
+           try now destruct (p (_ ,' eq_refl))
+       | _ => idtac
+       end.
+   all: apply it_eq_step in H; cbn in H; simp eval_aux in H.
+   all: dependent elimination H; cbn in r_rel; inversion_sigma r_rel as [ H1 H2 ].
+   all: revert m i H2; rewrite <- H1; intros m i H2; inversion_clear H2; cbn; clear.
+   all: econstructor; intros [ A p ] H; dependent elimination H; cbn in *.
+   all: dependent elimination v; [ apply it_eq_step in H; now inversion H | ].
+   4: dependent elimination w1; try now destruct (p0 (_ ,' eq_refl)).
+   1-3,5: dependent elimination w; try now destruct (p0 (_ ,' eq_refl)).   
+   all: apply it_eq_step in H; now inversion H .
 Qed.
 
-From OGS.OGS Require Spec.
+#[local] Instance sysL_typ  : baseT := {| typ := neg_ty |}.
 
-(*
-Definition ctx_allS (Γ : ctx neg_ty) : allS is_neg (c_map sub_elt Γ).
-  induction Γ; intros ? i; cbn in *.
-  - remember ∅%ctx as Γ; destruct i; inversion HeqΓ.
-  - remember (_ ▶ _)%ctx as Γ' in i; destruct i; inversion HeqΓ'.
-    + exact x.(sub_prf).
-    + rewrite <- H0 in IHΓ; exact (IHΓ _ i).
-Defined.
-
-Definition ctx_from (Γ : ctx neg_ty) : neg_ctx := {| sub_elt := c_map sub_elt Γ ; sub_prf := ctx_allS Γ |}.
-*)
-
-Definition mu_spec : Spec.interaction_spec :=
-  {| Spec.typ := neg_ty ;
-     Spec.msg := fun t => pat (t_neg t) ;
-     Spec.dom := fun t p => ctx_s_to (p_dom p) |}
-.
+#[local] Instance sysL_spec : observation_structure :=
+  {| obs A := pat (t_neg (neg_coe A)) ;
+     dom _ p := ctx_s_to (p_dom p) |} .
 
 Definition state' (Γ : ctx neg_ty) : Type := state (ctx_s_from Γ).
 Definition val' (Γ : ctx neg_ty) (a : neg_ty) : Type := val (ctx_s_from Γ) a.(sub_elt).
@@ -1948,28 +1695,19 @@ Definition to_nf {Γ} (u : nf (ctx_s_from Γ)) :
   sigT (fun t : neg_ty => prod (Γ ∋ t) (sigT (fun m : pat (t_neg t) => ctx_s_to (p_dom m) =[ val' ]> Γ ))) :=
   (_ ,' (to_has_L (fst (projT2 u)) , (projT1 (snd (projT2 u)) ,' to_FB (projT2 (snd (projT2 u)))))) .
 
-Program Definition mu_val : @Spec.lang_monoid mu_spec :=
-  {| Spec.val := val' ;
-     Spec.v_var := fun _ => ugly_var ;
-     Spec.v_sub := fun _ _ a _ v => v_subst (from_BB a) _ v ;
-  |}.
+#[local] Instance sysL_val  : baseV := {| Subst.val := val' |}.
+#[local] Instance sysL_conf : baseC := {| Subst.conf := state' |}.
 
-Program Definition mu_conf : @Spec.lang_module mu_spec mu_val :=
-  {| Spec.conf := state' ;
-     Spec.c_sub := fun _ _ a s => s_subst (from_BB a) s ;
-  |}.
+#[local] Instance sysL_val_mon : subst_monoid _ :=
+  {| v_var := @ugly_var ;
+     v_sub := fun _ _ a _ v => v_subst (from_BB a) _ v |} .
 
-Program Definition mu_machine : @Spec.machine mu_spec mu_val mu_conf :=
-  {| Spec.eval := fun _ c => fmap_delay to_nf (eval c) ;
-      Spec.app := fun _ _ v m r => p_app v m (from_FB r) |} .
-
-Lemma mu_val_laws : @Spec.lang_monoid_laws mu_spec mu_val .
-  unfold mu_spec, mu_val.
-  econstructor; unfold Spec.e_comp, s_map; cbn in *.
+#[local] Instance sysL_val_laws : subst_monoid_laws .
+  econstructor.
   - intros Γ Δ u1 u2 H1 i v1 v2 H2.
     apply v_sub_eq; auto.
     now rewrite H1.
-  - intros Γ1 Γ2 u ? i.
+  - intros Γ1 Γ2 u ? i; cbn.
     etransitivity.
     unfold ugly_var, from_has_L; apply v_sub_id_r.
     unfold from_BB, from_has_F, r_to_from_l, s_elt_upg, ctx_s_from, to_has_L.
@@ -1980,18 +1718,20 @@ Lemma mu_val_laws : @Spec.lang_monoid_laws mu_spec mu_val .
     etransitivity.
     apply v_sub_eq; [ apply from_BB_var | reflexivity ].
     apply v_sub_id_l.
-  - intros Γ1 Γ2 Γ3 Γ4 p q r ? i.
+  - intros Γ1 Γ2 Γ3 Γ4 p q r ? i; cbn.
     rewrite v_sub_sub.
     apply v_sub_eq; auto.
 Qed.
 
-Lemma mu_conf_laws : @Spec.lang_module_laws mu_spec mu_val mu_conf .
-  unfold mu_spec, mu_val, mu_conf.
-  econstructor; unfold Spec.e_comp, s_map; cbn in *.
+#[local] Instance sysL_conf_mod : subst_module _ _ :=
+  {| c_sub := fun _ _ a s => s_subst (from_BB a) s |} .
+
+#[local] Instance sysL_conf_laws : subst_module_laws .
+  econstructor.
   - intros Γ Δ u1 u2 H1 s1 s2 H2.
     apply s_sub_eq; auto.
     now rewrite H1.
-  - intros Γ c.
+  - intros Γ c; cbn.
     rewrite from_BB_var.
     apply s_sub_id_l.
   - intros Γ1 Γ2 Γ3 u v c; cbn.
@@ -1999,17 +1739,16 @@ Lemma mu_conf_laws : @Spec.lang_module_laws mu_spec mu_val mu_conf .
     apply s_sub_eq; auto.
 Qed.
 
-Lemma mu_var_laws : @Spec.var_assumptions mu_spec mu_val .
-  unfold mu_spec, mu_val.
-  econstructor; unfold Spec.is_var; cbn in *.
+#[local] Instance sysL_var_laws : var_assumptions.
+  econstructor.
   - exact @ugly_var_inj.
   - exact @ugly_var_dec.
   - exact @ugly_is_var_ren.
 Qed.
 
 Lemma to_comp_eq {Γ} (u v : delay (nf (ctx_s_from Γ))) (H : u ≋ v) :
-  @Spec.comp_eq mu_spec mu_val _ (fmap_delay to_nf u) (fmap_delay to_nf v) .
-  unfold Spec.comp_eq, fmap_delay.
+  Obs.comp_eq (fmap_delay to_nf u) (fmap_delay to_nf v) .
+  unfold Obs.comp_eq, fmap_delay.
   eapply (fmap_eq (RX := fun _ => nf_eq)); auto.
   intros [] ? ?  H1.
   destruct x as [ x1 [ i1 [ m1 γ1 ] ] ].
@@ -2035,14 +1774,16 @@ Definition to_pat {Γ : ctx neg_ty} : pat' (ctx_s_from Γ) -> sigT (fun x : neg_
   fun u => (_ ,' (to_has_L (fst (projT2 u)) , snd (projT2 u))) .
         
 Lemma from_to_pat_F {Γ : neg_ctx} (x y : nf (ctx_s_from (ctx_s_to Γ))) (H : x = y)
-  : from_pat_F (@Spec.msg_of_nf' mu_spec mu_val _ (to_nf x)) = pat_of_nf _ (n_rename r_from_to_l y) .
+  : from_pat_F (obs'_of_nf' _ (to_nf x)) = pat_of_nf _ (n_rename r_from_to_l y) .
   now rewrite H.
 Qed.
 
+#[local] Instance sysL_machine : machine :=
+  {| Machine.eval := fun _ c => fmap_delay to_nf (eval c) ;
+     Machine.app := fun _ _ v m e => p_app v m (from_FB e) |} .
 
-Definition mu_machine_laws : @Spec.machine_laws mu_spec mu_val mu_conf mu_machine.
-  unfold mu_spec, mu_val, mu_conf.
-  econstructor; unfold Spec.e_comp, s_map; cbn in *.
+#[local] Instance sysL_machine_law : machine_laws.
+  econstructor; unfold sysL_spec, sysL_val in *; cbn in *.
   - intros Γ x v m u1 u2 H.
     destruct x as [ [ [] | [] ] neg ]; cbn in *; try now destruct neg.
     all: do 2 f_equal; apply w_sub_eq; [ now rewrite H | reflexivity ].
@@ -2051,32 +1792,28 @@ Definition mu_machine_laws : @Spec.machine_laws mu_spec mu_val mu_conf mu_machin
     all: do 2 f_equal; change (w_subst ?u ?t) with (v_subst u t); rewrite v_sub_sub.
     all: apply v_sub_eq; auto.
   - intros Γ Δ c e .
-    unfold Spec.comp_eq, fmap_delay.
+    unfold Obs.comp_eq, fmap_delay.
     etransitivity.
     unshelve eapply fmap_eq. 5: exact (clean_hyp c (from_BB e)).
     exact ((fun _ => to_nf)).
     intros ? u v ->; unshelve econstructor; auto.
     unfold bind_delay', then_eval1.
     rewrite fmap_bind_com, bind_fmap_com.
-    apply (proj1 (t_gfp (it_eq_map ∅ₑ (fun _ : T1 => Spec.nf_eq')) _ _ _)).
+    apply (proj1 (t_gfp (it_eq_map ∅ₑ (fun _ : T1 => Obs.nf'_eq)) _ _ _)).
     eapply (it_eq_up2bind_t (eqᵢ _)); econstructor; auto.
     intros [] u v ->. 
-    change (gfp _ _ ?a ?b) with (Spec.comp_eq a b).
+    change (gfp _ _ ?a ?b) with (Obs.comp_eq a b).
     apply to_comp_eq.
     erewrite p_app_eq; auto.
     now rewrite <- (from_to_FB (projT2 (snd (projT2 v)))).
-  - intros Γ u .
-    unfold Spec.eval_to_msg, Spec.msg_of_nf', Spec.nf', Spec.nf_ty', Spec.nf_msg', Spec.nf_val', Spec.nf_var'.
-    destruct u as [ x [ j [ m γ ] ] ] ; cbn in *.
-    pose proof (eval_nf_ret ((x : ty) ,' (from_has_L j , (m ,' from_FB γ)))); cbn in H.
-    apply to_comp_eq in H.
-    rewrite H; clear H.
-    unfold Spec.comp_eq; apply it_eq_unstep; cbn; econstructor.
+  - intros Γ [ x [ j [ m γ ] ] ] ; cbn in *.
+    pose proof (eval_nf_ret ((x : ty) ,' (from_has_L j , (m ,' from_FB γ)))).
+    apply to_comp_eq in H; rewrite H; clear H.
+    unfold Obs.comp_eq; apply it_eq_unstep; cbn; econstructor.
     unshelve econstructor; auto; cbn.
     unshelve econstructor; auto; cbn.
     + exact (to_from_has_L _).
-    + unshelve econstructor; auto; cbn.
-      apply to_from_FB.
+    + unshelve econstructor; auto; cbn; apply to_from_FB.
   - intros [ [ t H ] p ]; simpl in p.
     pose (u := (t ,' p) : sigT (fun t : ty => pat (t_neg t))); simpl in u.
     change t with (projT1 u) in H |- *.
@@ -2089,14 +1826,14 @@ Definition mu_machine_laws : @Spec.machine_laws mu_spec mu_val mu_conf mu_machin
     eassert (H3 : _). refine (H0 ((projT1 y).(sub_elt) ,' projT2 y) _ ((projT1 y).(sub_prf))).
     * dependent elimination H2.
       cbn in *.
-      unfold Spec.eval_to_msg in i0.
+      unfold eval_to_obs in i0.
       destruct x as [ t m ]; cbn in *.
       unshelve econstructor.
       + clear - Γ ; exact (ctx_s_from Γ).
       + clear - v ; exact v.
       + clear - e ; exact (from_FB e).
       + exact (from_has_L i).
-      + intros []; apply p; unfold Spec.is_var, Spec.v_var.
+      + intros []; apply p; unfold Subst.is_var, v_var.
         apply (substS (fun u => sigT (fun i1 : Γ ∋ {| sub_elt := t; sub_prf := u |} => v = ugly_var {| sub_elt := t; sub_prf := u |} i1)) ((ctx_s_from Γ).(sub_prf) _ x)).
         refine (to_has_L x ,' _).
         rewrite e0; unfold ugly_var; f_equal; symmetry.
@@ -2105,7 +1842,7 @@ Definition mu_machine_laws : @Spec.machine_laws mu_spec mu_val mu_conf mu_machin
         eapply (fmap_eq (RY := eqᵢ _) (fun _ => from_pat_L) (fun _ => from_pat_L)) in i0; [ | intros ? ? ? ->; auto ].
         unfold fmap_delay in i0.
         rewrite 2 fmap_fmap_com in i0.
-        transitivity (((fun (_ : T1) (x : nf (ctx_s_from Γ)) => from_pat_L (@Spec.msg_of_nf' mu_spec mu_val Γ (to_nf x))) <$>
+        transitivity (((fun (_ : T1) (x : nf (ctx_s_from Γ)) => from_pat_L (obs'_of_nf' Γ (to_nf x))) <$>
         eval (p_app v m (from_FB e)))).
         unfold fmap_delay.
         eapply fmap_eq; auto.
@@ -2113,7 +1850,7 @@ Definition mu_machine_laws : @Spec.machine_laws mu_spec mu_val mu_conf mu_machin
            destruct n1 as [ x1 [ i1 [ m1 γ1 ]] ].
            destruct n2 as [ x2 [ i2 [ m2 γ2 ]] ].
            destruct H' as [ H2 [ H3 [ H4 _ ] ] ]; cbn in *.
-           unfold Spec.msg_of_nf', pat_of_nf, from_pat_L; cbn.
+           unfold Obs.obs'_of_nf', pat_of_nf, from_pat_L; cbn.
            revert i1 m1 γ1 H3 H4; rewrite H2; clear H2 x1; intros i1 m1 γ1 H3 H4; cbn in H3,H4.
            now rewrite H3, H4, from_to_has_L.
         ** rewrite i0; clear.
@@ -2125,30 +1862,19 @@ Definition mu_machine_laws : @Spec.machine_laws mu_spec mu_val mu_conf mu_machin
       reflexivity.
 Qed.
 
-Definition sem_act (Δ Γ : neg_ctx) : Type :=
-  @Spec.ogs_act mu_spec (ctx_s_to Δ) (∅ ▶ ctx_s_to Γ)%ctx .
-
-Definition sem_pas (Δ Γ : neg_ctx) : Type :=
-  @Spec.ogs_pas mu_spec (ctx_s_to Δ) (∅ ▶ ctx_s_to Γ)%ctx .
+Definition sem_act (Δ Γ : neg_ctx) : Type := ogs_act (ctx_s_to Δ) (∅ ▶ ctx_s_to Γ) .
+Definition sem_pas (Δ Γ : neg_ctx) : Type := ogs_pas (ctx_s_to Δ) (∅ ▶ ctx_s_to Γ) .
 
 Definition ugly_state {Γ : neg_ctx} (c : state Γ) : state (ctx_s_from (ctx_s_to Γ)) :=
   match ctx_s_to_inv (ctx_s_to Γ) as f in (fiber _ b) return (b = ctx_s_to Γ -> state (fib_extr f)) with
   | Fib a => fun H => rew <- [state ∘ coe_ctx] ctx_s_to_inj H in c
   end eq_refl .
 
-(*
-Definition interp_act {Δ Γ : neg_ctx} (c : state Γ) : sem_act Δ Γ :=
-  @Spec.m_strat mu_spec mu_val mu_conf mu_machine (ctx_s_to Δ) (∅ ▶ ctx_s_to Γ)%ctx
-    (@Spec.inj_init_act mu_spec mu_val mu_conf (ctx_s_to Δ) (ctx_s_to Γ)
-    (rew <- [state ∘ coe_ctx] ctx_s_from_to Γ in c)) .
-*)
-
 Definition from_to_state {Γ : neg_ctx} (c : state Γ) : state (ctx_s_from (ctx_s_to Γ)) :=
   s_rename r_from_to_r c .
 
 Definition interp_act_s Δ {Γ : neg_ctx} (c : state Γ) : sem_act Δ Γ :=
-  @Spec.m_strat mu_spec mu_val mu_conf mu_machine (ctx_s_to Δ) (∅ ▶ ctx_s_to Γ)%ctx
-    (@Spec.inj_init_act mu_spec mu_val mu_conf (ctx_s_to Δ) (ctx_s_to Γ) (from_to_state c)) .
+  m_strat (∅ ▶ ctx_s_to Γ) (inj_init_act (ctx_s_to Δ) (from_to_state c)) .
 Notation "⟦ t ⟧ₛ" := (interp_act_s _ t) .
 
 Definition ogs_weq_act Δ {Γ} : relation (sem_act Δ Γ) := fun u v => u ≈ v .
@@ -2163,15 +1889,13 @@ Definition subst_eq (Δ : neg_ctx) {Γ} : relation (state Γ) :=
 Theorem mu_subst_correct (Δ : neg_ctx) {Γ : neg_ctx} (x y : state Γ)
   : ⟦ x ⟧ₛ ≈[ Δ ]≈ ⟦ y ⟧ₛ -> subst_eq Δ x y .
   intros H σ.
-  apply (@Spec.ogs_correction mu_spec mu_val mu_val_laws mu_conf mu_conf_laws
-                 mu_var_laws mu_machine mu_machine_laws
-                 (ctx_s_to Γ)
-                 (ctx_s_to Δ)
-                 (from_to_state x)
-                 (from_to_state y)) in H.
-  specialize (H (to_FF σ)).
+  apply (ogs_correction (M := sysL_machine)
+            (ctx_s_to Δ)
+            (from_to_state x)
+            (from_to_state y)) in H.
 
-  unfold Spec.eval_in_env, Spec.eval_to_msg in H ; cbn in H.
+  specialize (H (to_FF σ)).
+  unfold eval_in_env, eval_to_msg, eval_to_obs in H; cbn in H.
 
   unshelve eapply (fmap_weq (RY := eqᵢ _) (fun _ : T1 => from_pat_F) (fun _ : T1 => from_pat_F) _ _ _ _) in H.
   intros [] ? ? ->; auto.
@@ -2198,7 +1922,7 @@ Notation "⟦ t ⟧ₚ" := (interp_act_s _ (c_of_t_p t)) .
 
 Definition a_of_sk_p {Γ Δ : neg_ctx} {x : ty0 pos} (s : Γ =[val]> Δ) (k : term Δ (t- x))
   : (Γ ▶ₛ {| sub_elt := t- x ; sub_prf := stt |}) =[val]> Δ :=
-  s_append s (k : val Δ (t- x)) .
+  a_append s (k : val Δ (t- x)) .
 
 Lemma sub_csk_p {Γ Δ : neg_ctx} {x : ty0 pos} (t : term Γ (t+ x)) (s : Γ =[val]> Δ) (k : term Δ (t- x))
               : Cut _ (t_subst s _ t) k = s_subst (a_of_sk_p s k) (c_of_t_p t) .
@@ -2228,7 +1952,7 @@ Notation "⟦ t ⟧ₙ" := (interp_act_s _ (c_of_t_n t)) .
 
 Definition a_of_sk_n {Γ Δ : neg_ctx} {x : ty0 neg} (s : Γ =[val]> Δ) (k : term Δ (t+ x))
   : (Γ ▶ₛ {| sub_elt := t+ x ; sub_prf := stt |}) =[val]> Δ :=
-  s_append s (k : val Δ (t+ x)) .
+  a_append s (k : val Δ (t+ x)) .
 
 Lemma sub_csk_n {Γ Δ : neg_ctx} {x : ty0 neg} (t : term Γ (t- x)) (s : Γ =[val]> Δ) (k : term Δ (t+ x))
               : Cut _ k (t_subst s _ t) = s_subst (a_of_sk_n s k) (c_of_t_n t) .
